src/Ex/Mesi/MesiInv.v
@@ -1,0 +1,119 @@
+Require Import Bool List String Peano_dec Lia.
+Require Import Common FMap IndexSupport HVector Syntax Topology Semantics SemFacts StepM.
+Require Import Invariant TrsInv Simulation Serial SerialFacts.
+Require Import RqRsLang RqRsCorrect.
+
+Require Import Ex.Spec Ex.SpecInds Ex.Template.
+Require Import Ex.Mesi Ex.Mesi.Mesi Ex.Mesi.MesiTopo.
+
+Set Implicit Arguments.
+
+Import PropMonadNotations.
+Import CaseNotations.
+
+Local Open Scope list.
+Local Open Scope hvec.
+Local Open Scope fmap.
+
+(* NOTE: these ltacs only work for constants (channels, objects, etc.),
+ * thus will be used only in this file.
+ *)
+(* Ltac get_lock_minds oidx := *)
+(*   progress (good_footprint_get oidx); *)
+(*   repeat (repeat disc_rule_conds_unit_simpl; try disc_footprints_ok); *)
+(*   disc_minds_const. *)
+ 
+(* Ltac get_lock_inv obj sys := *)
+(*   let H := fresh "H" in *)
+(*   assert (In obj (sys_objs sys)) as H by (simpl; tauto); *)
+(*   progress (good_locking_get obj); *)
+(*   clear H. *)
+
+Existing Instance Mesi.ImplOStateIfc.
+
+Definition MsgExistsSig (sig: MSig) (msgs: MessagePool Msg) :=
+  exists idm, InMPI msgs idm /\ sigOf idm = sig.
+
+Section Inv.
+
+  Section ObjUnit.
+    Variables (oidx: IdxT)
+              (orq: ORq Msg)
+              (ost: OState)
+              (msgs: MessagePool Msg).
+
+    Definition MsgNotRsI (idm: Id Msg) :=
+      match case (sigOf idm) on sig_dec default True with
+        |! (downTo oidx, (MRs, mesiRsI)): False
+      end.
+
+    Definition NoRsI :=
+      forall idm, InMPI msgs idm -> MsgNotRsI idm.
+
+    Definition ImplOStateMESI (cv: nat): Prop :=
+      mesiS <= ost#[implStatusIdx] -> NoRsI ->
+      ost#[implValueIdx] = cv.
+
+    Definition NotCohMsg (idm: Id Msg) :=
+      match case (sigOf idm) on sig_dec default True with
+      | (downTo oidx, (MRs, mesiRsS)): False
+      | (downTo oidx, (MRs, mesiRsE)): False
+      | (rsUpFrom oidx, (MRs, mesiDownRsS)): False
+      end.
+
+    Definition NoCohMsgs :=
+      forall idm, InMPI msgs idm -> NotCohMsg idm.
+
+    Definition CohRqI :=
+      forall idm,
+        InMPI msgs idm ->
+        sigOf idm = (rqUpFrom oidx, (MRq, mesiRqI)) ->
+        msg_value (valOf idm) = ost#[implValueIdx].
+
+    Definition ObjExcl0 :=
+      mesiE <= ost#[implStatusIdx] /\ NoRsI /\ NoCohMsgs /\ CohRqI.
+
+    Definition ObjExcl :=
+      ObjExcl0 \/
+      MsgExistsSig (downTo oidx, (MRs, mesiRsE)) msgs \/
+      MsgExistsSig (downTo oidx, (MRs, mesiRsM)) msgs.
+
+    Definition ObjInvalid0 :=
+      ost#[implStatusIdx] = mesiI /\ NoCohMsgs.
+
+    Definition ObjInvalid :=
+      ObjInvalid0 \/
+      MsgExistsSig (downTo oidx, (MRs, mesiRsI)) msgs.
+
+    Section Facts.
+
+      Lemma NoRsI_MsgExistsSig_false:
+        MsgExistsSig (downTo oidx, (MRs, mesiRsI)) msgs ->
+        NoRsI -> False.
+      Proof.
+        intros.
+        destruct H as [idm [? ?]].
+        specialize (H0 _ H).
+        red in H0; rewrite H1 in H0.
+        unfold caseDec in H0.
+        find_if_inside; auto.
+      Qed.
+
+    End Facts.
+    
+  End ObjUnit.
+
+  Definition InvExcl (st: MState): Prop :=
+    forall eidx,
+      eost <+- (bst_oss st)@[eidx];
+        (ObjExcl eidx eost (bst_msgs st) ->
+         forall oidx,
+           oidx <> eidx ->
+           ost <+- (bst_oss st)@[oidx];
+             ObjInvalid oidx ost (bst_msgs st)).
+
+End Inv.
+
+Hint Unfold NoRsI ImplOStateMESI ObjExcl0 ObjExcl
+     NoCohMsgs CohRqI ObjInvalid0 ObjInvalid: RuleConds.
+
